theories/SpecNotations.v
@@ -1,5 +1,11 @@
 Require Import Blech.Spec.
 
+Bind Scope list_scope with environment.
+Bind Scope list_scope with subst.
+Bind Scope list_scope with vars.
+Bind Scope list_scope with usage.
+Bind Scope list_scope with spans.
+
 Infix "*" := t_prod.
 
 Notation "G ⊢ v 'in' t" := (Jv G v t) (at level 90).
